transfered some notes

ExistentialRules/ChaseSequence/Core.lean
@@ -4,6 +4,9 @@ import ExistentialRules.Models.Cores
 import PossiblyInfiniteTrees.PossiblyInfiniteTree.FiniteDegreeTree.Basic
 import ExistentialRules.Models.Basic
 import ExistentialRules.Triggers.Basic
+import ExistentialRules.AtomsAndFacts.Basic
+import ExistentialRules.AtomsAndFacts.SubstitutionsAndHomomorphisms
+
 
 variable {sig : Signature} [DecidableEq sig.P] [DecidableEq sig.C] [DecidableEq sig.V]
 variable {obs : ObsoletenessCondition sig} {kb : KnowledgeBase sig}
@@ -13,3 +16,74 @@ def ChaseNode.isWeakCore {obs : ObsoletenessCondition sig} (node : ChaseNode obs
 
 def ChaseNode.isStrongCore {obs : ObsoletenessCondition sig} (node : ChaseNode obs rules) :
  Prop := FactSet.isStrongCore node.fact.val
+
+------
+
+def GroundTermMapping.applyMapSetFactSet (hs : Set (GroundTermMapping sig)) (fs : FactSet sig) : true := sorry
+
+def ChaseBranch.applyMapSetFactSetEqApplyFactSetSeq (hs : Set (GroundTermMapping sig)) (fs : FactSet sig) : true := sorry
+
+
+structure TGD extends Rule sig where
+  -- define structure of TGDs here
+  p1 : true
+  p2 : true
+
+structure EGD extends Rule sig where
+ -- define structure of EGDs here
+  p1 : true
+  p2 : true
+
+def Rule.stratified (a b : Rule sig) : Prop := sorry
+-- b
+infixr:50 " ≺ " => Rule.stratified
+
+def RuleSet.isWeaklyAcyclic : Prop := sorry
+
+theorem weaklyAcycIfStratified (rs : RuleSet sig) : RuleSet.isWeaklyAcyclic → ∀ r ∈ rs, r.isStratified := by sorry
+
+
+-- theorem 7
+theorem ExUniversalModelIffCoreChaseHasModel : true := sorry
+
+infixr:65 " ⊧ " => FactSet.modelsKb
+infixr:65 " ⊧ " => FactSet.modelsDb
+infixr:65 " ⊧ " => FactSet.modelsRule
+infixr:65 " ⊧ " => FactSet.modelsRules
+infixr:65 " ⊧ᵤ" => FactSet.universallyModelsKb
+
+-- if A ⊧ R(x) ↔ B ⊧ R(h x)
+def GroundTermMapping.isFull (h : GroundTermMapping sig) : Prop := sorry
+
+-- h is full injective hom.
+def GroundTermMapping.isEmbedding (h : GroundTermMapping sig) : Prop := sorry
+
+-- should we define hom indepndent of GTMs ?
+
+-- r : A → B ⊆ A, e is the id on dom(B)
+def GroundTermMapping.isRetract (h : GroundTermMapping sig) : Prop := sorry
+
+def GroundTermmapping.isProperRetract (h : GroundTermMapping sig) : Prop := sorry
+  -- h.isRetract ∧ ¬ h.surjective
+
+-- if the body is machted return the head with applied h else do nothing
+-- => we maybe should split this into a Rule.apply that always applies and a Rule.isActive
+--    which returns a prop whenever the body can be matched
+-- => ExistentialRules.ChaseSequence.Universality.lean
+-- es gibt bereits GTM.isHomomorphism
+def Rule.apply (r : Rule sig) (h : GroundTermMapping sig) (fs : FactSet sig) : FactSet sig := sorry
+
+-- cores calculation is only neccessary after finitely many steps
+theorem CoreCalcAfterFiniteEq : true := sorry
+
+def FactSet.isFClosedFor (F : Set (GroundTermMapping sig)) (T : FactSet sig) (K : FactSet sig) : Prop := sorry
+
+-- needs refinement
+abbrev ModelSet := Set (FactSet sig)
+
+-- U must be finite, K cannot
+def isUniversalSetModel (U : Set (FactSet sig)) (K : Set (FactSet sig)) (F : Set (GroundTermMapping sig)) :
+  ∀ M ∈ K, ∃ T ∈ U, FactSet.isFClosedFor F T M ∧
+  U ⊆ K ∧
+  U.finite ∧
+  ¬ ∃ U' ⊂ U, isUniversalSetModel U' U F := by sorry
